commit proof

messageInvariantPrototypes/toyLeaderElection/centralized/applicationProof.dfy
@@ -10,11 +10,39 @@ import opened Obligations
 *                                Application Invariants                                *
 ***************************************************************************************/
 
+// Application Invariant: Host having a vote implies voter nominated that host
+ghost predicate HasVoteImpliesVoterNominates(c: Constants, v: Variables)
+  requires v.WF(c)
+{
+  forall nominee: nat, voter: nat | 
+    && c.ValidHostId(nominee)
+    && c.ValidHostId(voter)
+    && v.hosts[nominee].HasVoteFrom(voter)
+  ::
+    v.hosts[voter].Nominates(nominee)
+}
+
+ghost predicate ReceivedVotesValid(c: Constants, v: Variables)
+  requires v.WF(c)
+{
+  forall h: nat | c.ValidHostId(h)
+  :: v.hosts[h].receivedVotes <= (set x | 0 <= x < |c.hostConstants|)
+}
+
+ghost predicate IsLeaderImpliesHasQuorum(c: Constants, v: Variables)
+  requires v.WF(c)
+{
+  forall h: nat | c.ValidHostId(h) && v.IsLeader(c, h)
+  :: SetIsQuorum(c.hostConstants[h].clusterSize, v.hosts[h].receivedVotes)
+}
+
 // Application bundle
 ghost predicate ApplicationInv(c: Constants, v: Variables)
   requires v.WF(c)
 {
-  true
+  && ReceivedVotesValid(c, v)
+  && IsLeaderImpliesHasQuorum(c, v)  // this says that the set size doesn't shrink
+  && HasVoteImpliesVoterNominates(c, v)
 }
 
 ghost predicate Inv(c: Constants, v: Variables)
@@ -43,8 +71,78 @@ lemma InvInductive(c: Constants, v: Variables, v': Variables)
   requires Inv(c, v)
   requires Next(c, v, v')
   ensures Inv(c, v')
+{
+  IsLeaderImpliesHasQuorumInductive(c, v, v');
+  SafetyProof(c, v');
+}
+
+lemma ReceivedVotesValidInductive(c: Constants, v: Variables, v': Variables) 
+  requires Inv(c, v)
+  requires Next(c, v, v')
+  ensures ReceivedVotesValid(c, v')
 {}
 
-
-
+lemma IsLeaderImpliesHasQuorumInductive(c: Constants, v: Variables, v': Variables) 
+  requires Inv(c, v)
+  requires Next(c, v, v')
+  requires ReceivedVotesValid(c, v')
+  ensures IsLeaderImpliesHasQuorum(c, v')
+{
+  var allHosts := (set x | 0 <= x < |c.hostConstants|);
+  forall h: nat | c.ValidHostId(h) && v'.IsLeader(c, h)
+  ensures
+    && SetIsQuorum(c.hostConstants[h].clusterSize, v'.hosts[h].receivedVotes)
+  {
+    var step :| NextStep(c, v, v', step);
+    if step.HostLocalStep? {
+      var actor := step.host;
+      assert c.ValidHostId(actor);
+      var lbl := Host.InternalLbl();
+      var hc := c.hostConstants[actor];
+      var hv, hv' := v.hosts[actor], v'.hosts[actor];
+      assert Host.Next(c.hostConstants[actor], v.hosts[actor], v'.hosts[actor], lbl);
+      var hostStep :| Host.NextStep(hc, hv, hv', hostStep, lbl);
+      if hostStep.HostStep? {
+        // trigger
+        assert SetIsQuorum(c.hostConstants[h].clusterSize, v'.hosts[h].receivedVotes);
+      } else if hostStep.VictoryStep? {
+        if !v.IsLeader(c, h) {
+          // triggers
+          assert v'.hosts[h].receivedVotes == v.hosts[h].receivedVotes;
+          assert SetIsQuorum(hc.clusterSize, hv.receivedVotes);
+        }
+      } 
+    } else if step.VoteStep? {
+      // trigger
+      assert SetIsQuorum(c.hostConstants[h].clusterSize, v'.hosts[h].receivedVotes);
+    }
+  }
 }
+
+lemma SafetyProof(c: Constants, v': Variables)
+  requires v'.WF(c)
+  requires ReceivedVotesValid(c, v')
+  requires IsLeaderImpliesHasQuorum(c, v')
+  requires HasVoteImpliesVoterNominates(c, v')
+  ensures Safety(c, v')
+{
+  /* Proof by contradiction: Assume two leaders were elected in v', L1 and L2.
+  * Then by quorum intersection, there is a common rogueId in both L1.receivedVotes and
+  * L2.receivedVotes. This violates HasVoteImpliesVoterNominates
+  */
+  if !Safety(c, v') {
+    var l1: nat :| c.ValidHostId(l1) && v'.IsLeader(c, l1);
+    var l2: nat :| c.ValidHostId(l2) && v'.IsLeader(c, l2) && l2 != l1;
+    var clusterSize := |c.hostConstants|;
+    var allHosts := (set x | 0 <= x < |c.hostConstants|);
+    SetComprehensionSize(|c.hostConstants|);
+
+    var rv1, rv2 :=  v'.hosts[l1].receivedVotes, v'.hosts[l2].receivedVotes;
+    var rogueId := QuorumIntersection(allHosts, rv1, rv2);  // witness
+
+    assert v'.hosts[rogueId].nominee == Some(l1);  // trigger
+    assert v'.hosts[rogueId].nominee == Some(l2);  // trigger
+    assert false;
+  }
+}
+} // end module ToyLeaderElectionProof
